src/impl/TLS13.Impl.Driver.PairingProtectedReplay.fsti
@@ -20,6 +20,86 @@ module Seq = FStar.Seq
 module W = TLS13.Wire.Spec
 module WFL = TLS13.Spec.WireFormatLemmas
 
+noextract
+let paired_handshake_complete_boundary_state_logs
+  (client:CS.connection_state)
+  (server:CS.connection_state)
+  (start:CS.handshake_start)
+  (ch:M.client_hello)
+  (selection:CS.server_handshake_selection)
+  (server_shared:C.x25519_shared_secret)
+  (client_shared:C.x25519_shared_secret)
+  (sh:M.server_hello)
+  (server_material:CS.traffic_key_material)
+  (client_material:CS.traffic_key_material)
+  (sent_msg0:M.handshake_msg)
+  (received_msg0:M.handshake_msg)
+  (sent_msg1:M.handshake_msg)
+  (received_msg1:M.handshake_msg)
+  (server_auth_skip:CS.local_event)
+  (client_auth_skip:CS.local_event)
+  (sent_msg2:M.handshake_msg)
+  (received_msg2:M.handshake_msg)
+  (client_verify_skip:CS.local_event)
+  (sent_msg3:M.handshake_msg)
+  (received_msg3:M.handshake_msg)
+  (verified_server_finished:M.finished)
+  (client_app_write_material:CS.traffic_key_material)
+  (client_app_read_material:CS.traffic_key_material)
+  (server_app_write_material:CS.traffic_key_material)
+  (sent_msg4:M.handshake_msg)
+  (received_msg4:M.handshake_msg)
+  : prop =
+  let server_suffix =
+    PWL.server_protected_handshake_contiguous_replay_events
+      server_material
+      sent_msg0
+      sent_msg1
+      server_auth_skip
+      sent_msg2
+      sent_msg3
+      server_app_write_material
+      received_msg4
+      [] in
+  let client_suffix =
+    PWL.client_protected_handshake_contiguous_replay_events
+      client_material
+      received_msg0
+      received_msg1
+      client_auth_skip
+      received_msg2
+      client_verify_skip
+      received_msg3
+      verified_server_finished
+      client_app_write_material
+      client_app_read_material
+      sent_msg4
+      [] in
+  let server_prefix =
+    PWSeg.server_cleartext_handshake_prefix_events
+      ch
+      selection
+      server_shared
+      sh in
+  let client_prefix =
+    PWSeg.client_cleartext_handshake_prefix_events
+      start
+      ch
+      sh
+      client_shared in
+  Seq.equal
+    server.CS.cs_wire_log.CL.raw_sent
+    client.CS.cs_wire_log.CL.raw_received /\
+  Seq.equal
+    client.CS.cs_wire_log.CL.raw_sent
+    server.CS.cs_wire_log.CL.raw_received /\
+  server.CS.cs_event_log == FStar.List.Tot.append server_prefix server_suffix /\
+  client.CS.cs_event_log == FStar.List.Tot.append client_prefix client_suffix /\
+  CS.connection_state_sent_seal_replay_consistent server /\
+  CS.connection_state_received_decode_replay_consistent server /\
+  CS.connection_state_sent_seal_replay_consistent client /\
+  CS.connection_state_received_decode_replay_consistent client
+
 val lemma_client_server_application_record_material_agrees_from_cleartext_raw_and_contiguous_replay_views
   (client:CS.connection_state)
   (server:CS.connection_state)
@@ -736,6 +816,372 @@ val lemma_client_server_application_record_material_agrees_from_cleartext_prefix
           client_full_sent
           client_full_received
           client_final))
+      (ensures
+        CS.supported_profile_client_server_key_material_agrees client server /\
+        CS.peer_record_material_agrees
+          (CS.traffic_id CS.TrafficApplication CS.ClientTraffic)
+          client
+          server /\
+        CS.peer_record_material_agrees
+          (CS.traffic_id CS.TrafficApplication CS.ServerTraffic)
+          client
+          server)
+
+val lemma_client_server_application_record_material_agrees_from_handshake_complete_boundary
+  (client:CS.connection_state)
+  (server:CS.connection_state)
+  (client_ch:M.client_hello)
+  (server_ch:M.client_hello)
+  (client_sh:M.server_hello)
+  (server_sh:M.server_hello)
+  (client_ch_raw:B.bytes)
+  (server_ch_raw:B.bytes)
+  (client_sh_raw:B.bytes)
+  (server_sh_raw:B.bytes)
+  (start:CS.handshake_start)
+  (selection:CS.server_handshake_selection)
+  (server_shared:C.x25519_shared_secret)
+  (client_shared:C.x25519_shared_secret)
+  (server_model1:CS.connection_model)
+  (server_model2:CS.connection_model)
+  (server_model3:CS.connection_model)
+  (server_model4:CS.connection_model)
+  (server_model5:CS.connection_model)
+  (client_model1:CS.connection_model)
+  (client_model2:CS.connection_model)
+  (client_model3:CS.connection_model)
+  (client_model4:CS.connection_model)
+  (server_after_install:CS.connection_model)
+  (client_after_install:CS.connection_model)
+  (server_after0:CS.connection_model)
+  (client_after0:CS.connection_model)
+  (server_after1:CS.connection_model)
+  (client_after1:CS.connection_model)
+  (server_after_auth_skip:CS.connection_model)
+  (client_after_auth_skip:CS.connection_model)
+  (server_after2:CS.connection_model)
+  (client_after2:CS.connection_model)
+  (client_after_verify_skip:CS.connection_model)
+  (server_after3:CS.connection_model)
+  (client_after3:CS.connection_model)
+  (server_auth_skip:CS.local_event)
+  (client_auth_skip:CS.local_event)
+  (client_verify_skip:CS.local_event)
+  (server_material:CS.traffic_key_material)
+  (client_material:CS.traffic_key_material)
+  (sent_msg0:M.handshake_msg)
+  (received_msg0:M.handshake_msg)
+  (sent_msg1:M.handshake_msg)
+  (received_msg1:M.handshake_msg)
+  (sent_msg2:M.handshake_msg)
+  (received_msg2:M.handshake_msg)
+  (sent_msg3:M.handshake_msg)
+  (received_msg3:M.handshake_msg)
+  (verified_server_finished:M.finished)
+  (client_app_write_material:CS.traffic_key_material)
+  (client_app_read_material:CS.traffic_key_material)
+  (server_app_write_material:CS.traffic_key_material)
+  (sent_msg4:M.handshake_msg)
+  (received_msg4:M.handshake_msg)
+  (cf_client_after_verify:CS.connection_model)
+  (cf_client_after_app_write:CS.connection_model)
+  (cf_client_after_app_read:CS.connection_model)
+  (cf_server_after_app_write:CS.connection_model)
+  (cf_client_after_finished:CS.connection_model)
+  (cf_server_after_finished:CS.connection_model)
+  : Lemma
+      (requires (
+        let server_model0 =
+          CS.initial_model server.CS.cs_model.CS.model_config in
+        let client_model0 =
+          CS.initial_model client.CS.cs_model.CS.model_config in
+        CD.client_driver_application_ready client /\
+        SD.server_driver_application_ready server /\
+        client.CS.cs_model.CS.model_handshake.CS.hs_client_hello == Some client_ch /\
+        server.CS.cs_model.CS.model_handshake.CS.hs_client_hello == Some server_ch /\
+        client.CS.cs_model.CS.model_handshake.CS.hs_server_hello == Some client_sh /\
+        server.CS.cs_model.CS.model_handshake.CS.hs_server_hello == Some server_sh /\
+        server_ch == client_ch /\
+        client_sh == server_sh /\
+        WFL.supported_client_hello_wire_profile client_ch /\
+        Seq.equal client_ch_raw server_ch_raw /\
+        Seq.equal server_sh_raw client_sh_raw /\
+        CS.cleartext_tls_message_raw
+          (M.TlsHandshake (M.ClientHello client_ch))
+          client_ch_raw /\
+        CS.received_cleartext_tls_message_raw
+          (M.TlsHandshake (M.ClientHello server_ch))
+          server_ch_raw /\
+        CS.cleartext_tls_message_raw
+          (M.TlsHandshake (M.ServerHello server_sh))
+          server_sh_raw /\
+        CS.received_cleartext_tls_message_raw
+          (M.TlsHandshake (M.ServerHello client_sh))
+          client_sh_raw /\
+        W.parse_supported_server_hello
+          (W.serialize_handshake (M.ServerHello server_sh)) == Some server_sh /\
+        W.parse_supported_server_hello
+          (W.serialize_handshake (M.ServerHello client_sh)) == Some client_sh /\
+        Pairing.client_server_driver_first_epoch_no_key_update_state_inputs
+          client
+          server /\
+        paired_handshake_complete_boundary_state_logs
+          client
+          server
+          start
+          client_ch
+          selection
+          server_shared
+          client_shared
+          server_sh
+          server_material
+          client_material
+          sent_msg0
+          received_msg0
+          sent_msg1
+          received_msg1
+          server_auth_skip
+          client_auth_skip
+          sent_msg2
+          received_msg2
+          client_verify_skip
+          sent_msg3
+          received_msg3
+          verified_server_finished
+          client_app_write_material
+          client_app_read_material
+          server_app_write_material
+          sent_msg4
+          received_msg4 /\
+        CS.step_model
+          server_model0
+          (CS.ConnLocalEvent CS.LocalStartServer) == Some server_model1 /\
+        CS.step_model
+          server_model1
+          (CS.ConnNetworkEvent {
+            CL.message_direction = CL.Received;
+            CL.message_value = M.TlsHandshake (M.ClientHello client_ch);
+          }) == Some server_model2 /\
+        CS.step_model
+          server_model2
+          (CS.ConnLocalEvent (CS.LocalSelectServerParameters selection)) ==
+          Some server_model3 /\
+        CS.step_model
+          server_model3
+          (CS.ConnLocalEvent (CS.LocalDeriveSharedSecret server_shared)) ==
+          Some server_model4 /\
+        CS.step_model
+          server_model4
+          (CS.ConnNetworkEvent {
+            CL.message_direction = CL.Sent;
+            CL.message_value = M.TlsHandshake (M.ServerHello server_sh);
+          }) == Some server_model5 /\
+        CS.step_model
+          client_model0
+          (CS.ConnLocalEvent (CS.LocalStartHandshake start)) ==
+          Some client_model1 /\
+        CS.step_model
+          client_model1
+          (CS.ConnNetworkEvent {
+            CL.message_direction = CL.Sent;
+            CL.message_value = M.TlsHandshake (M.ClientHello client_ch);
+          }) == Some client_model2 /\
+        CS.step_model
+          client_model2
+          (CS.ConnNetworkEvent {
+            CL.message_direction = CL.Received;
+            CL.message_value = M.TlsHandshake (M.ServerHello server_sh);
+          }) == Some client_model3 /\
+        CS.step_model
+          client_model3
+          (CS.ConnLocalEvent (CS.LocalDeriveSharedSecret client_shared)) ==
+          Some client_model4 /\
+        (match
+          client.CS.cs_model.CS.model_handshake.CS.hs_encrypted_extensions,
+          server.CS.cs_model.CS.model_handshake.CS.hs_encrypted_extensions,
+          client.CS.cs_model.CS.model_handshake.CS.hs_certificate,
+          server.CS.cs_model.CS.model_handshake.CS.hs_certificate,
+          client.CS.cs_model.CS.model_handshake.CS.hs_certificate_verify,
+          server.CS.cs_model.CS.model_handshake.CS.hs_certificate_verify,
+          client.CS.cs_model.CS.model_handshake.CS.hs_server_finished,
+          server.CS.cs_model.CS.model_handshake.CS.hs_server_finished,
+          client.CS.cs_model.CS.model_handshake.CS.hs_client_finished,
+          server.CS.cs_model.CS.model_handshake.CS.hs_client_finished
+        with
+        | Some client_ee, Some server_ee_msg,
+          Some client_cert, Some server_cert_msg,
+          Some client_cv, Some server_cv_msg,
+          Some client_sf, Some server_sf,
+          Some client_cf, Some server_cf ->
+          sent_msg0 == M.EncryptedExtensions server_ee_msg /\
+          received_msg0 == M.EncryptedExtensions client_ee /\
+          sent_msg1 == M.Certificate server_cert_msg /\
+          received_msg1 == M.Certificate client_cert /\
+          sent_msg2 == M.CertificateVerify server_cv_msg /\
+          received_msg2 == M.CertificateVerify client_cv /\
+          sent_msg3 == M.Finished server_sf /\
+          received_msg3 == M.Finished client_sf /\
+          sent_msg4 == M.Finished client_cf /\
+          received_msg4 == M.Finished server_cf
+        | _, _, _, _, _, _, _, _, _, _ ->
+          False) /\
+        (match
+          server_model5.CS.model_handshake.CS.hs_keys.CS.ks_handshake_secret,
+          client_model4.CS.model_handshake.CS.hs_keys.CS.ks_handshake_secret
+        with
+        | Some server_secret, Some client_secret ->
+          Seq.equal server_secret client_secret
+        | _, _ ->
+          False) /\
+        Seq.equal
+          server_model5.CS.model_handshake.CS.hs_transcript
+          client_model4.CS.model_handshake.CS.hs_transcript /\
+        PWL.local_event_does_not_install_record_keys server_auth_skip /\
+        PWL.local_event_does_not_install_record_keys client_auth_skip /\
+        PWL.local_event_does_not_install_record_keys client_verify_skip /\
+        PWL.write_read_record_material_aligned client_model4 server_model5 /\
+        PWL.protected_handshake_wire_round_trip_message sent_msg0 /\
+        PWL.protected_handshake_wire_round_trip_message received_msg0 /\
+        PWL.protected_handshake_wire_round_trip_message sent_msg1 /\
+        PWL.protected_handshake_wire_round_trip_message received_msg1 /\
+        PWL.protected_handshake_wire_round_trip_message sent_msg2 /\
+        PWL.protected_handshake_wire_round_trip_message received_msg2 /\
+        PWL.protected_handshake_wire_round_trip_message sent_msg3 /\
+        PWL.protected_handshake_wire_round_trip_message received_msg3 /\
+        PWL.protected_handshake_wire_round_trip_message sent_msg4 /\
+        PWL.protected_handshake_wire_round_trip_message received_msg4 /\
+        CS.step_model
+          server_model5
+          (CS.ConnLocalEvent
+            (CS.LocalInstallTrafficKeysForRole {
+              CS.install_role = CS.ServerEndpoint;
+              CS.install_payload = {
+                CS.install_epoch = CS.TrafficHandshake;
+                CS.install_direction = CS.TrafficWrite;
+                CS.install_material = server_material;
+              };
+            })) == Some server_after_install /\
+        CS.step_model
+          client_model4
+          (CS.ConnLocalEvent
+            (CS.LocalInstallTrafficKeys {
+              CS.install_epoch = CS.TrafficHandshake;
+              CS.install_direction = CS.TrafficRead;
+              CS.install_material = client_material;
+            })) == Some client_after_install /\
+        CS.step_model
+          server_after_install
+          (CS.ConnNetworkEvent {
+            CL.message_direction = CL.Sent;
+            CL.message_value = M.TlsHandshake sent_msg0;
+          }) == Some server_after0 /\
+        CS.step_model
+          client_after_install
+          (CS.ConnNetworkEvent {
+            CL.message_direction = CL.Received;
+            CL.message_value = M.TlsHandshake received_msg0;
+          }) == Some client_after0 /\
+        server_after0.CS.model_record.CS.record_write ==
+          R.next_seq server_after_install.CS.model_record.CS.record_write /\
+        client_after0.CS.model_record.CS.record_read ==
+          R.next_seq client_after_install.CS.model_record.CS.record_read /\
+        CS.step_model
+          server_after0
+          (CS.ConnNetworkEvent {
+            CL.message_direction = CL.Sent;
+            CL.message_value = M.TlsHandshake sent_msg1;
+          }) == Some server_after1 /\
+        CS.step_model
+          client_after0
+          (CS.ConnNetworkEvent {
+            CL.message_direction = CL.Received;
+            CL.message_value = M.TlsHandshake received_msg1;
+          }) == Some client_after1 /\
+        server_after1.CS.model_record.CS.record_write ==
+          R.next_seq server_after0.CS.model_record.CS.record_write /\
+        client_after1.CS.model_record.CS.record_read ==
+          R.next_seq client_after0.CS.model_record.CS.record_read /\
+        CS.step_model server_after1 (CS.ConnLocalEvent server_auth_skip) ==
+          Some server_after_auth_skip /\
+        CS.step_model client_after1 (CS.ConnLocalEvent client_auth_skip) ==
+          Some client_after_auth_skip /\
+        CS.step_model
+          server_after_auth_skip
+          (CS.ConnNetworkEvent {
+            CL.message_direction = CL.Sent;
+            CL.message_value = M.TlsHandshake sent_msg2;
+          }) == Some server_after2 /\
+        CS.step_model
+          client_after_auth_skip
+          (CS.ConnNetworkEvent {
+            CL.message_direction = CL.Received;
+            CL.message_value = M.TlsHandshake received_msg2;
+          }) == Some client_after2 /\
+        server_after2.CS.model_record.CS.record_write ==
+          R.next_seq server_after_auth_skip.CS.model_record.CS.record_write /\
+        client_after2.CS.model_record.CS.record_read ==
+          R.next_seq client_after_auth_skip.CS.model_record.CS.record_read /\
+        CS.step_model client_after2 (CS.ConnLocalEvent client_verify_skip) ==
+          Some client_after_verify_skip /\
+        CS.step_model
+          server_after2
+          (CS.ConnNetworkEvent {
+            CL.message_direction = CL.Sent;
+            CL.message_value = M.TlsHandshake sent_msg3;
+          }) == Some server_after3 /\
+        CS.step_model
+          client_after_verify_skip
+          (CS.ConnNetworkEvent {
+            CL.message_direction = CL.Received;
+            CL.message_value = M.TlsHandshake received_msg3;
+          }) == Some client_after3 /\
+        server_after3.CS.model_record.CS.record_write ==
+          R.next_seq server_after2.CS.model_record.CS.record_write /\
+        client_after3.CS.model_record.CS.record_read ==
+          R.next_seq client_after_verify_skip.CS.model_record.CS.record_read /\
+        CS.step_model
+          client_after3
+          (CS.ConnLocalEvent (CS.LocalVerifyFinished verified_server_finished)) ==
+          Some cf_client_after_verify /\
+        CS.step_model
+          cf_client_after_verify
+          (CS.ConnLocalEvent
+            (CS.LocalInstallTrafficKeys {
+              CS.install_epoch = CS.TrafficApplication;
+              CS.install_direction = CS.TrafficWrite;
+              CS.install_material = client_app_write_material;
+            })) == Some cf_client_after_app_write /\
+        CS.step_model
+          cf_client_after_app_write
+          (CS.ConnLocalEvent
+            (CS.LocalInstallTrafficKeys {
+              CS.install_epoch = CS.TrafficApplication;
+              CS.install_direction = CS.TrafficRead;
+              CS.install_material = client_app_read_material;
+            })) == Some cf_client_after_app_read /\
+        CS.step_model
+          server_after3
+          (CS.ConnLocalEvent
+            (CS.LocalInstallTrafficKeysForRole {
+              CS.install_role = CS.ServerEndpoint;
+              CS.install_payload = {
+                CS.install_epoch = CS.TrafficApplication;
+                CS.install_direction = CS.TrafficWrite;
+                CS.install_material = server_app_write_material;
+              };
+            })) == Some cf_server_after_app_write /\
+        CS.step_model
+          cf_client_after_app_read
+          (CS.ConnNetworkEvent {
+            CL.message_direction = CL.Sent;
+            CL.message_value = M.TlsHandshake sent_msg4;
+          }) == Some cf_client_after_finished /\
+        CS.step_model
+          cf_server_after_app_write
+          (CS.ConnNetworkEvent {
+            CL.message_direction = CL.Received;
+            CL.message_value = M.TlsHandshake received_msg4;
+          }) == Some cf_server_after_finished))
       (ensures
         CS.supported_profile_client_server_key_material_agrees client server /\
         CS.peer_record_material_agrees
